Progress in sharpening simple connections filter

src/packet_filters.v
@@ -57,6 +57,28 @@ Definition FilterMethod (r: QueryStructure PacketHistorySchema) (inp: input) : C
     ((OutgoingToRule inp.(in_ip4).(SourceAddress)).(cf_cond) pre = true)) };
     if b then ret (Some ACCEPT) else ret (Some DROP).
 
+Definition FilterMethod_UnConstr (r: UnConstrQueryStructure PacketHistorySchema) (inp: input) : Comp (option result) :=
+  if (OutgoingRule.(cf_cond) inp) then ret (Some ACCEPT)
+  else if negb (IncomingRule.(cf_cond) inp) then ret None
+  else b <- { b: bool | decides b (exists pre,
+    IndexedEnsemble_In (GetUnConstrRelation r Fin.F1) < sINPUT :: pre > /\
+    ((OutgoingToRule inp.(in_ip4).(SourceAddress)).(cf_cond) pre = true)) };
+    if b then ret (Some ACCEPT) else ret (Some DROP).
+
+Lemma UnConstrPreservesFilterMethod: forall r_o r_n inp res,
+  DropQSConstraints_AbsR r_o r_n ->
+  computes_to (FilterMethod r_o inp) res <->
+  computes_to (FilterMethod_UnConstr r_n inp) res.
+Proof.
+  intros. unfold FilterMethod, FilterMethod_UnConstr in *.
+  destruct (OutgoingRule.(cf_cond) inp) eqn:out. reflexivity.
+  destruct (negb (IncomingRule.(cf_cond) inp)) eqn:inc. reflexivity.
+  split; intros; apply Bind_inv in H0; destruct H0 as [b [Hbin Hbres]];
+    unfold DropQSConstraints_AbsR in H; rewrite <- H in *; computes_to_econstructor;
+    [rewrite GetRelDropConstraints; apply Hbin | apply Hbres
+    | rewrite <- GetRelDropConstraints; apply Hbin | apply Hbres].
+Qed.
+
 Definition NoIncomingConnectionsFilter : ADT StatefulFilterSig :=
   Eval simpl in Def ADT {
     rep := QueryStructure PacketHistorySchema,
@@ -68,25 +90,190 @@ Definition NoIncomingConnectionsFilter : ADT StatefulFilterSig :=
       ret (r, res)
   }%methDefParsing.
 
-Definition LessHistoryRelation (r_o r_n : QueryStructure PacketHistorySchema) :=
+Lemma simpl_in_bind:
+  forall (T U: Type) (x v : T) (y: U),
+    In T (`(r', _) <- ret (x, y); ret r') v -> x = v.
+Proof.
+  intros. apply Bind_inv in H. destruct H. destruct H. apply Return_inv in H. rewrite <- H in H0. simpl in H0. apply Return_inv in H0. assumption. Qed.
+
+Definition UnIndexedEnsembleListEquivalence'
+           (ElementType : Type)
+           (ensemble : IndexedEnsemble)
+           (l : list ElementType) :=
+  sig (fun (l': list IndexedElement) =>
+         map indexedElement l' = l /\
+         (forall x : IndexedElement,
+            In IndexedElement ensemble x <-> List.In x l') /\
+         NoDup (map elementIndex l')).
+
+
+Definition AllFinite {qs_schema} (r: UnConstrQueryStructure qs_schema) :=
+  forall idx, {l: list RawTuple & UnIndexedEnsembleListEquivalence' _ (GetUnConstrRelation r idx) l}.
+
+Definition FiniteTables_AbsR'
+    {qs_schema}
+    (r_o : UnConstrQueryStructure qs_schema)
+    (r_n : { r_n: UnConstrQueryStructure qs_schema & AllFinite r_n }) :=
+  r_o = projT1 r_n.
+
+Lemma QSEmptyIsFinite {qs_schema}: AllFinite (DropQSConstraints (QSEmptySpec qs_schema)).
+Proof.
+  unfold AllFinite. intros. exists []. exists [].
+  split. reflexivity. split. split; intros.
+(*  pose proof (FiniteEnsemble_QSEmptySpec idx) as Hfin. red in Hfin.
+  destruct Hfin as [l Hl]. red in Hl. destruct Hl as [l' [Hmap [Heqv Hdup]]]. *)
+  unfold In, GetUnConstrRelation, DropQSConstraints, QSEmptySpec in H. simpl in H.
+
+
+  Coercion mycoer {qs_schema idx t}
+           (y: @IndexedElement
+                 (@RawTuple
+                    (@GetNRelSchemaHeading
+                       (numRawQSschemaSchemas
+                          (QueryStructureSchemaRaw qs_schema))
+                       (qschemaSchemas (QueryStructureSchemaRaw qs_schema)) idx))) :
+    @IndexedRawTuple
+      (rawSchemaHeading
+         (@Vector.nth RawSchema (numQSschemaSchemas qs_schema) t idx)).
+  Admitted.
+
+  assert (Hscraw: qschemaSchemas qs_schema = Vector.map schemaRaw (QSschemaSchemas qs_schema)).
+  { reflexivity. }
+
+  replace x with (@mycoer _ _ (@Vector.map Schema RawSchema schemaRaw (numQSschemaSchemas _) (QSschemaSchemas _)) x) in H.
+  rewrite <- Hscraw in H. rewrite <- ith_imap2 in H.
+  Set Printing All. Check (Build_EmptyRelation_IsEmpty qs_schema idx). simpl in H. admit. admit.
+  (*replace (fun ns: RawSchema => RawRelation ns) with RawRelation in H. rewrite Build_EmptyRelation_IsEmpty in H.*)
+  inversion H. constructor.
+Qed.
+Unset Printing All.
+
+Lemma FiniteTables_AbsR'_QSEmptySpec
+      {qs_schema}
+  :  FiniteTables_AbsR'
+       (DropQSConstraints (QSEmptySpec qs_schema))
+       (existT AllFinite (DropQSConstraints (QSEmptySpec qs_schema)) QSEmptyIsFinite).
+Proof. reflexivity. Qed.
+
+Lemma change_refine_form {X1 X2 Y Z} :
+  forall (cx: Comp (X1 * X2)) (cy: X1 * X2 -> Comp Y) (f: Y -> Comp Z),
+    refine
+      (x <- cx;
+       y <- cy x;
+       f y)
+      (x0 <- (x <- cx;
+              y <- cy x;
+              ret (y, snd x));
+       f (fst x0)).
+Proof.
+  intros.
+  unfold refine; intros.
+  computes_to_inv; subst.
+  eauto.
+Qed.
+
+
+Lemma insert_finite_helper:
+  forall (qs_schema : RawQueryStructureSchema)
+         (r_n: { r_n: UnConstrQueryStructure qs_schema & AllFinite r_n })
+         idx tup,
+    UnConstrFreshIdx (GetUnConstrRelation (projT1 r_n) idx) (elementIndex tup) ->
+    AllFinite (UpdateUnConstrRelation (projT1 r_n) idx
+                 (EnsembleInsert tup (GetUnConstrRelation (projT1 r_n) idx))).
+Proof.
+  red; intros qsc r_n idx tup Hfresh idx'. destruct (Fin.eqb idx idx') eqn:idxeq.
+  - apply Fin.eqb_eq in idxeq. subst idx'.
+    destruct r_n as [r Hfin]. destruct (Hfin idx) as [l1 Hl1].
+    destruct Hl1 as [l2 [Hmap [Hin Hdup]]].
+    exists ((indexedElement tup) :: l1). cbn.
+    rewrite get_update_unconstr_eq. red. exists (tup :: l2).
+    
+    split. simpl. rewrite <- Hmap. reflexivity. split.
+    split; intros H; unfold EnsembleInsert, In in *;
+      destruct H; simpl;
+        [ left; symmetry; assumption
+        | right; apply (Hin x); apply H
+        | left; symmetry; assumption
+        | right; apply (Hin x); apply H].
+    
+    simpl. apply NoDup_cons. red in Hfresh. simpl in Hfresh.
+    assert (Hlist: forall (x: nat) l,
+               (forall x', List.In x' l -> lt x' x) ->
+               ~List.In x l).
+    {
+      intros x l Hx'. intro Hx. apply (Hx' x) in Hx.
+      apply lt_irrefl in Hx. inversion Hx.
+    }
+    apply Hlist. apply forall_In_map. intros elem Helem.
+    apply Hfresh. apply (Hin elem).
+    assumption. assumption.
+    
+  - assert (Hidxeq: idx <> idx').
+    { intro. apply Fin.eqb_eq in H. congruence. }
+    destruct r_n as [r Hfin]. destruct (Hfin idx') as [l1 Hl1].
+    exists l1. cbn. rewrite get_update_unconstr_neq.
+    assumption. assumption.
+Qed.
+
+Lemma FiniteTables_AbsR'_Insert :
+  forall (qs_schema : RawQueryStructureSchema) r_o r_n
+         (idx : Fin.t (numRawQSschemaSchemas qs_schema)) tup,
+    FiniteTables_AbsR' r_o r_n ->
+    UnConstrFreshIdx (ith2 r_o idx) (elementIndex tup) ->
+    forall (H: UnConstrFreshIdx (GetUnConstrRelation (projT1 r_n) idx) (elementIndex tup)),
+    refine
+      {r_n0 : { r_n: UnConstrQueryStructure qs_schema & AllFinite r_n } |
+       FiniteTables_AbsR'
+         (UpdateUnConstrRelation r_o idx (EnsembleInsert tup (GetUnConstrRelation r_o idx))) r_n0}
+      (ret (existT AllFinite
+              (UpdateUnConstrRelation (projT1 r_n) idx
+                 (EnsembleInsert tup (GetUnConstrRelation (projT1 r_n) idx)))
+              (insert_finite_helper _ _ _ _ H))).
+Proof.
+  intros qsc r_o r_n idx tup Hrel Hfresho Hfreshn.
+  unfold refine; intros r_n' Hr_n'. apply Return_inv in Hr_n'. subst r_n'.
+  computes_to_econstructor. red; cbn. red in Hrel. subst r_o. reflexivity.
+Qed.
+
+
+Definition LessHistoryRelation (r_o r_n : sigT (@AllFinite PacketHistorySchema)) :=
   forall inp,
     (OutgoingRule.(cf_cond) inp) ->
-    ((IndexedEnsemble_In (GetRelation r_n Fin.F1) < sINPUT :: inp >)
-     <-> IndexedEnsemble_In (GetRelation r_o Fin.F1) < sINPUT :: inp >).
+    ((IndexedEnsemble_In (GetUnConstrRelation (projT1 r_n) Fin.F1) < sINPUT :: inp >)
+     <-> IndexedEnsemble_In (GetUnConstrRelation (projT1 r_o) Fin.F1) < sINPUT :: inp >).
 
 Lemma LessHistoryPreservesFilter:
-  forall inp r_o r_n val,
+  forall inp r_o r_n,
     LessHistoryRelation r_o r_n ->
-    computes_to (FilterMethod r_o inp) val ->
-    computes_to (FilterMethod r_n inp) val.
+    refine
+      (FilterMethod_UnConstr (projT1 r_o) inp)
+      (FilterMethod_UnConstr (projT1 r_n) inp).
 Proof.
-  intros. unfold FilterMethod in *. unfold LessHistoryRelation in H.
-  destruct (cf_cond OutgoingRule inp) eqn:outrule. apply H0.
-  destruct (negb (cf_cond IncomingRule inp)) eqn:ninrule; simpl in *. apply H0.
-  inversion H0. destruct H1. computes_to_econstructor. destruct x eqn:truefalse. assert (Hsol: computes_to { b: bool | decides b (exists pre: input, IndexedEnsemble_In (GetRelation r_n Fin.F1) (icons2 pre inil2) /\ cf_cond (OutgoingToRule (SourceAddress (in_ip4 inp))) pre = true) } true).
-  { computes_to_econstructor. unfold decides; simpl. destruct H1. destruct H1. exists x0. split. apply (H x0). apply (OutgoingToImpliesOutgoing x0 (SourceAddress (in_ip4 inp))). apply H3. apply H1. apply H3. } apply Hsol.
-  computes_to_econstructor; unfold decides; simpl. unfold not; intros. destruct H1. destruct H3. destruct H1. exists x0. split. apply (H x0). apply (OutgoingToImpliesOutgoing x0 (SourceAddress (in_ip4 inp))). apply H3. apply H1. apply H3.
-  apply H2.
+  red; intros. unfold FilterMethod_UnConstr in *.
+  unfold LessHistoryRelation in H.
+  destruct (cf_cond OutgoingRule inp) eqn:outrule;
+    destruct (negb (cf_cond IncomingRule inp)) eqn:ninrule;
+    simpl in *; try apply H0.
+  inversion H0. destruct H1. computes_to_econstructor.
+  destruct x eqn:truefalse.
+
+  - instantiate (1 := x).
+    computes_to_econstructor. unfold decides; simpl.
+    destruct H1. destruct H1. exists x0. split.
+    * apply (H x0).
+      apply (OutgoingToImpliesOutgoing x0 (SourceAddress (in_ip4 inp))).
+      assumption. assumption.
+    * assumption.
+
+  - computes_to_econstructor; unfold decides; simpl.
+    unfold not; intros. destruct H1. destruct H3. destruct H1.
+    exists x0. split.
+    * apply (H x0).
+      apply (OutgoingToImpliesOutgoing x0 (SourceAddress (in_ip4 inp))).
+      assumption. assumption.
+    * assumption.
+
+  - assumption.
 Qed.
 
 
@@ -95,31 +282,23 @@ Lemma LessHistoryRelationRefl:
 Proof.
   unfold LessHistoryRelation; split; intros; assumption. Qed.
 
-Lemma SimplInBind:
-  forall (T U: Type) (x v : T) (y: U),
-    In T (`(r', _) <- ret (x, y); ret r') v -> x = v.
-Proof.
-  intros. apply Bind_inv in H. destruct H. destruct H. apply Return_inv in H. rewrite <- H in H0. simpl in H0. apply Return_inv in H0. assumption. Qed.
+Definition IncrMaxFreshIdx (r: sigT (@AllFinite PacketHistorySchema)) :=
+  S (fold_right (fun elem acc => max (elementIndex elem) acc) 0 (proj1_sig (projT2 ((projT2 r) Fin.F1)))).
 
-Print FiniteTables_AbsR. Check QSInsertSpec_refine_opt.
-
-Print LessHistoryRelation.
-
-Lemma InsertIfOutgoingRefinesFilter:
-  forall (r_o: QueryStructure PacketHistorySchema) d,
+Lemma IncrMaxFreshIdx_Refine:
+  forall (r: sigT (@AllFinite PacketHistorySchema)),
     refine
-      (r <- QSInsert r_o Fin.F1 (icons2 d inil2);
-       {r_n0 : QueryStructure PacketHistorySchema |
-            LessHistoryRelation (fst r) r_n0})
-      (r <- if cf_cond OutgoingRule d
-                  then QSInsert r_o Fin.F1 (icons2 d inil2)
-                  else ret (r_o, true);
-       ret (fst r)).
+      {idx: nat | UnConstrFreshIdx (GetUnConstrRelation (projT1 r) Fin.F1) idx}
+      (ret (IncrMaxFreshIdx r)).
 Proof.
-  intros. destruct (cf_cond OutgoingRule d) eqn:outd; unfold refine; intros.
-  - inversion H. destruct H0. computes_to_econstructor. apply H0. computes_to_econstructor. rewrite H1. apply LessHistoryRelationRefl.
-  - pose proof (SimplInBind _ _ r_o v _ H). rewrite <- H0. subst. computes_to_econstructor. apply QSInsertSpec_refine_opt. simpl. computes_to_econstructor. unfold UnConstrFreshIdx. computes_to_econstructor. intros. Admitted.
-    
+  intros r. pose (proj2_sig (projT2 ((projT2 r) Fin.F1))) as Hl.
+  destruct Hl as [Hmap [Heqv Hdup]].
+  intro idx; intro Hidx; computes_to_econstructor;
+    intro elem; intros Helem.
+  apply Return_inv in Hidx. apply Heqv in Helem.
+  unfold lt. rewrite <- Hidx. apply le_n_S.
+  apply fold_right_max_is_max; apply Helem.
+Qed.
 
 
 Theorem SharpenNoIncomingFilter:
@@ -127,7 +306,6 @@ Theorem SharpenNoIncomingFilter:
 Proof.
   start sharpening ADT.
   hone representation using (@DropQSConstraints_AbsR PacketHistorySchema).
-
   - apply Constructor_DropQSConstraints.
   - simplify with monad laws.
     unfold Bind2.
@@ -135,137 +313,98 @@ Proof.
     Transparent QSInsert.
     cbn.
 
-    + etransitivity.
-      eapply refine_bind.
-      reflexivity.
-      unfold pointwise_relation.
-      intros.
+    etransitivity.
+    eapply refine_bind.
+    reflexivity.
+    unfold pointwise_relation.
+    intros.
 
-      Lemma urgh {X1 X2 Y Z} :
-        forall (cx: Comp (X1 * X2)) (cy: X1 * X2 -> Comp Y) (f: Y -> Comp Z),
-          refine
-            (x <- cx;
-             y <- cy x;
-             f y)
-            (x0 <- (x <- cx;
-                   y <- cy x;
-                   ret (y, snd x));
-             f (fst x0)).
-      Proof.
-        intros.
-        unfold refine; intros.
-        computes_to_inv; subst.
-        eauto.
-      Qed.
-
-      etransitivity.
-      apply urgh.
-      unfold QSInsert.
-      rewrite QSInsertSpec_UnConstr_refine; eauto; cycle 1.
-      * refine pick val true.
-        reflexivity.
-        exact I.
-      * refine pick val true.
-        reflexivity.
-        cbv; intros; exact I.
-      * refine pick val true.
-        reflexivity.
-        cbv; intros; exact I.
-      * cbv -[refine].
-        refine pick val true.
-        simplify with monad laws.
-        reflexivity.
-        exact I.
-      * cbv -[refine].
-        intros; refine pick val true.
-        simplify with monad laws.
-        higher_order_reflexivity.
-        eauto.
+    etransitivity.
+    apply change_refine_form.
+    unfold QSInsert.
+    rewrite QSInsertSpec_UnConstr_refine; eauto; cycle 1;
+      try (refine pick val true; [reflexivity | cbv; intros; exact I]);
+      try (cbv -[refine]; intros; refine pick val true;
+        [simplify with monad laws; higher_order_reflexivity | eauto]).
       * simplify with monad laws.
         higher_order_reflexivity.
-      * Axiom FilterMethod_UnConstr :
-          UnConstrQueryStructure PacketHistorySchema -> input -> Comp (option result).
-        replace (FilterMethod r_o d) with (FilterMethod_UnConstr r_n d) by admit.
-        subst H.
-        higher_order_reflexivity.
+      * etransitivity. eapply refine_bind. red; intros v Htemp.
+        apply (UnConstrPreservesFilterMethod r_o r_n d v H0). apply Htemp.
+        unfold pointwise_relation; intros. higher_order_reflexivity.
+        subst H. higher_order_reflexivity.
 
-  -
-    Definition AllFinite {qs_schema} (r: UnConstrQueryStructure qs_schema) :=
-      forall idx, (FiniteEnsemble (GetUnConstrRelation r idx)).
-    
-    Definition FiniteTables_AbsR'
-               {qs_schema}
-               (r_o : UnConstrQueryStructure qs_schema)
-               (r_n : { r_n: UnConstrQueryStructure qs_schema | AllFinite r_n }) :=
-      r_o = proj1_sig r_n.
-
-    hone representation using (@FiniteTables_AbsR' PacketHistorySchema).
+  - hone representation using (@FiniteTables_AbsR' PacketHistorySchema).
     + simplify with monad laws.
-      unshelve refine pick val (exist _ (DropQSConstraints (QSEmptySpec _)) _).
-      * admit.
-      * subst H.
-        higher_order_reflexivity.
-      * reflexivity.
+      refine pick val
+        (existT _ (DropQSConstraints (QSEmptySpec _)) QSEmptyIsFinite).
+      * subst H; higher_order_reflexivity.
+      * apply FiniteTables_AbsR'_QSEmptySpec.
     + simplify with monad laws.
       eapply refine_bind.
-      * red in H0.
-        subst.
+      * red in H0; simpl in H0; rewrite H0.
         higher_order_reflexivity.
-      * red; intros.
-        Axiom pick_idx :
-          forall  {ElementType: Type} e,
-            FiniteEnsemble e ->
-            { idx: nat & @UnConstrFreshIdx ElementType e idx }.
-
-        red in H0.
-        subst.
-
-        refine pick val (projT1 (pick_idx _ ((proj2_sig r_n) Fin.F1))); [ | eauto using (projT2 (pick_idx _ ((proj2_sig r_n) Fin.F1))) ].
-
-        simplify with monad laws.
-        cbn.
-
-        Axiom urgh2 :
-          forall (qs_schema : RawQueryStructureSchema)
-            (r_n: { r_n: UnConstrQueryStructure qs_schema | AllFinite r_n })
-            idx tup,
-            AllFinite (UpdateUnConstrRelation (`r_n) idx (EnsembleInsert tup (GetUnConstrRelation (`r_n) idx))).
-        
-        Axiom FiniteTables_AbsR'_Insert :
-          forall (qs_schema : RawQueryStructureSchema) (r_o : UnConstrQueryStructure qs_schema)
-            r_n
-            (idx : Fin.t (numRawQSschemaSchemas qs_schema)) (tup : IndexedElement),
-            FiniteTables_AbsR' r_o r_n ->
-            UnConstrFreshIdx (ith2 r_o idx) (elementIndex tup) ->
-            refine
-              {r_n0 : { r_n: UnConstrQueryStructure qs_schema | AllFinite r_n } |
-               FiniteTables_AbsR'
-                 (UpdateUnConstrRelation r_o idx (EnsembleInsert tup (GetUnConstrRelation r_o idx))) r_n0}
-              (ret (exist
-                          AllFinite
-                          (UpdateUnConstrRelation (`r_n) idx
-                                                  (EnsembleInsert tup (GetUnConstrRelation (`r_n) idx)))
-                          (urgh2 _ _ _ _))).
-
+      * red; intros. red in H0. subst r_o.
+        eapply refine_under_bind_both.
+        apply IncrMaxFreshIdx_Refine.
+        intros idx Hidx; cbn.
         rewrite FiniteTables_AbsR'_Insert; cbn; eauto.
-        simplify with monad laws.
+        simplify with monad laws. higher_order_reflexivity.
+        unfold FiniteTables_AbsR'. reflexivity.
 
-        Focus 2.
-        unfold FiniteTables_AbsR'.
+    + hone representation using LessHistoryRelation;
+        try simplify with monad laws.
+      * refine pick val
+          (existT _ (DropQSConstraints (QSEmptySpec _)) QSEmptyIsFinite).
+        subst H; reflexivity. apply LessHistoryRelationRefl.
+      * etransitivity. eapply refine_under_bind.
+        intros res Hres. cbn. eapply refine_bind.
+
+        Definition RefinedInsert
+                   (r: sigT (@AllFinite PacketHistorySchema)) d H :=
+          existT AllFinite (UpdateUnConstrRelation (projT1 r) Fin.F1
+            (EnsembleInsert
+               {| elementIndex := IncrMaxFreshIdx r;
+                  indexedElement := icons2 d inil2 |}
+               (GetUnConstrRelation (projT1 r) Fin.F1)))
+            (insert_finite_helper PacketHistorySchema r Fin.F1
+               {| elementIndex := IncrMaxFreshIdx r;
+                  indexedElement := icons2 d inil2 |} H).
+        
+        refine pick val
+               (if cf_cond OutgoingRule d
+                then (RefinedInsert r_n d _)
+                else r_n).
         reflexivity.
-        higher_order_reflexivity.
 
-        admit.
-        admit.
+        destruct (cf_cond OutgoingRule d) eqn:outrule.
+        red; intros inp Hinp. unfold RefinedInsert. split; intros.
+
+        cbn in H1. rewrite get_update_unconstr_eq in H1. red in H1. destruct H1. destruct H1.
+        { exists (IncrMaxFreshIdx r_o). cbn. red. rewrite get_update_unconstr_eq. red. left. inversion H1. reflexivity. }
+        { cbn. rewrite get_update_unconstr_eq. red. unfold In. unfold EnsembleInsert. pose proof (H0 inp Hinp). unfold IndexedEnsemble_In in H2. unfold In in H2. assert (Hm: exists idx, GetUnConstrRelation (projT1 r_o) Fin.F1 {| elementIndex := idx; indexedElement := icons2 (value (ilist2_hd (icons2 (sINPUT :: inp)%Component inil2))) inil2 |}). { apply H2. exists x. apply H1. } destruct Hm. exists x0. right. apply H3. }
+
+        cbn in H1. rewrite get_update_unconstr_eq in H1. red in H1. destruct H1. destruct H1.
+        { exists (IncrMaxFreshIdx r_n). cbn. red. rewrite get_update_unconstr_eq. red. left. inversion H1. reflexivity. }
+        { cbn. rewrite get_update_unconstr_eq. red. unfold In. unfold EnsembleInsert. pose proof (H0 inp Hinp). unfold IndexedEnsemble_In in H2. unfold In in H2. assert (Hm: exists idx, GetUnConstrRelation (projT1 r_n) Fin.F1 {| elementIndex := idx; indexedElement := icons2 (value (ilist2_hd (icons2 (sINPUT :: inp)%Component inil2))) inil2 |}). { apply H2. exists x. apply H1. } destruct Hm. exists x0. right. apply H3. }
+
+        red; intros inp Hinp. split; intros.
+
+        apply (H0 inp Hinp) in H1. cbn. rewrite get_update_unconstr_eq. red. red in H1. destruct H1. exists x. red. red. right. apply H1.
+
+        cbn in H1; rewrite get_update_unconstr_eq in H1. red in H1. destruct H1. red in H1. red in H1. destruct H1. inversion H1. rewrite <- H4 in outrule. rewrite outrule in Hinp. inversion Hinp. apply (H0 inp Hinp). red; exists x; red. apply H1.
+
+
+        red; intros. higher_order_reflexivity.
+        simplify with monad laws. eapply refine_bind.
+        apply (LessHistoryPreservesFilter d r_o r_n H0).
+        red; intros. higher_order_reflexivity.
+
+
+      * 
+        
+
 
         
-        
-  hone representation using LessHistoryRelation; try simplify with monad laws.
-  - refine pick val (QSEmptySpec PacketHistorySchema). unfold refine. intros. Transparent computes_to. apply H0. unfold LessHistoryRelation. intros. split; intros; inversion H1; inversion H2.
-  - unfold Bind2. simplify with monad laws. cbn. Check InsertIfOutgoingRefinesFilter.
-    
-
-
 (*
 Definition sID := "ID".
 Definition sPACKET := "Packet".
